commands and assertions

theories/commands.v
@@ -6,6 +6,7 @@ From Coq Require Import Init.Nat.
 From Coq Require Import Arith.Arith.
 From Coq Require Import Arith.EqNat. Import Nat.
 Require Import  Coq.Logic.JMeq.
+From Coq Require Import Logic.PropExtensionality.
 
 Record exec_model_consts : Type := make_exec_model_consts
   {
@@ -34,10 +35,18 @@ Record exec_model_theory (E : exec_model_consts) : Prop := make_emt
   (* Preservation of monad bind*)
   preserve_bind1 : forall (A B: Type) (f : A -> (M E) B) (x y : (M E) A) 
   (Hxy : exec_partial E A x y),
-    exists Hbind,
-    bind E (ap (bop E A) x y Hxy) f = ap (bop E B) (bind E x f) (bind E y f) Hbind;
-  preserve_bind2 : forall (A B : Type) (f : A -> (M E) B) (x : (M E) A),
+    exists H,
+    bind E (ap (bop E A) x y Hxy) f = ap (bop E B) (bind E x f) (bind E y f) H;
+  preserve_bind2 : forall (A B : Type) (f : A -> (M E) B),
     bind E (id E A) f = id E B ;
+
+  (* Need to find a good way to formalize this rule to require that 
+     f + g is defined *)
+  preserve_bind3 : forall (A B : Type) (f g : A -> (M E) B) (x : (M E) A)
+    (Hfg : forall (y : A), exec_partial E B (f y) (g y)),
+    exists H,
+    ap (bop E B) (bind E x f) (bind E x g) H = 
+    bind E x (fun y => ap (bop E B) (f y) (g y) (Hfg y));
   
   (* Monad Laws *)
   bind_with_unit : forall (A : Type) (m : (M E) A),
@@ -65,6 +74,16 @@ Proof.
   - subst. easy.
 Qed.
 
+Theorem pcm_id_comm : forall (E : exec_model_consts) (Ext: exec_model_theory E) 
+  (A : Type) (x : (M E) A), 
+  exists (Hx : exec_partial E A (id E A) x), ap (bop E A) (id E A) x Hx = x.
+Proof.
+  intros. assert (forall Hx, exists H', ap (bop E A) x (id E A) Hx = ap (bop E A) (id E A) x H').
+    { intros. apply (pcm_comm E Ext). }
+  assert (exists Hx, ap (bop E A) x (id E A) Hx = x ).
+    { apply (pcm_id E Ext). }
+  inversion H0. specialize (H x0). inversion H. exists x1. rewrite <- H2. apply H1.
+Qed.
 
 (* Before defining the syntax and semantics of the command language, we define
    program states and semantics for a language of atomic commands on those 
@@ -143,35 +162,22 @@ Definition veval (st : state) (v : vexp) : val :=
   end.
 
 (* Syntax and Semantics for atomic commands *)
-Inductive CAtomic : Type :=
+Inductive CAtomic (Ex : exec_model_consts): Type :=
  | CAssume (e : vexp)
  | CAsgn (x : string) (v : vexp).
 
-Definition ceval_atomic (Ex : exec_model_consts) (st : state) (c : CAtomic) : (M Ex state) :=
+Definition ceval_atomic (Ex : exec_model_consts) (st : state) (c : CAtomic Ex) : (M Ex state) :=
   match c with
-  | CAssume e => match veval st e with
-                  | Bval true => unit Ex st
-                  | _ => id Ex state
+  | CAssume _ e => match veval st e with
+                  | Bval false => id Ex state
+                  | _ => unit Ex st
                   end
-  | CAsgn x v => let st' := fun x' => if String.eqb x x' then (veval st v) else (st x') in
+  | CAsgn _ x v => let st' := fun x' => if String.eqb x x' then (veval st v) else (st x') in
                   unit Ex st'
                  end.
+          
 
-(* Defining the command language *)
-Inductive com : Type :=
-  | CDiv
-  | CSkip 
-  | CSeq (c1 c2 : com)
-  | CPlus (c1 c2 : com)
-  | CAtom (c : CAtomic).
-
-
-Definition compatible (Ex : exec_model_consts) (e1 e2 : vexp) : Prop :=
-  forall st : state, exists He x, 
-  ap (bop Ex val) (unit Ex (veval st e1)) (unit Ex (veval st e2)) He = x.
-
-
-Definition compatible' (e1 e2 : vexp) : Prop :=
+Definition compatible (e1 e2 : vexp) : Prop :=
   forall st : state,
   (veval st e1 = Bval false) \/ (veval st e2 = Bval false).
 
@@ -180,8 +186,12 @@ Definition is_total (Ex : exec_model_consts) : Prop :=
   forall (A : Type) (x y : M Ex A),
   exec_partial Ex A x y.
   
+(* The below is a failed attempt at ceval where we tried to define it by inducting
+    on a proof of well-formed-ness of commands, but this ended up being too 
+    complicated when trying to do proofs involving ceval as it made it harder 
+    to simpl things. *)
 
-Inductive wf_com (Ex : exec_model_consts) :  com -> Type :=
+(* Inductive wf_com (Ex : exec_model_consts) :  com -> Type :=
   | wf_div : wf_com Ex CDiv
   | wf_skip : wf_com Ex CSkip
   | wf_seq : forall (c1 c2 : com), 
@@ -189,7 +199,7 @@ Inductive wf_com (Ex : exec_model_consts) :  com -> Type :=
   | wf_plus_total : forall (c1 c2 : com), 
       is_total Ex -> wf_com Ex c1 -> wf_com Ex c2 -> wf_com Ex (CPlus c1 c2)
   | wf_plus : forall (e1 e2 : vexp) (c1 c2 : com), 
-      compatible' e1 e2 -> wf_com Ex c1 -> 
+      compatible e1 e2 -> wf_com Ex c1 -> 
       wf_com Ex c2 -> 
       wf_com Ex (CPlus (CSeq (CAtom (CAssume e1)) c1) (CSeq (CAtom (CAssume e2)) c2))
   | wf_atom : forall (c : CAtomic), wf_com Ex (CAtom c).
@@ -210,56 +220,174 @@ Program Fixpoint ceval (Ex : exec_model_consts) (Ext : exec_model_theory Ex)
     | Bval false => (ceval Ex Ext c2 st wf2) 
     | _ => (ceval Ex Ext c1 st wf1)
     end
+  end. *)
+
+(* Below, we try to define the denotational semantics w/o needing a proof of 
+   well-formed-ness of commands *)
+
+(* Note that the CPlus (non-total case) definition is implicitly
+    (Assume e1 ; c1) + (Assume e2 ; c2 ) *)
+Inductive com (Ex : exec_model_consts) : Type :=
+  | CDiv
+  | CSkip 
+  | CSeq (c1 c2 : com Ex)
+  | CPlus_total (c1 c2 : com Ex) (pf : is_total Ex)
+  | CPlus (e1 e2 : vexp) (c1 c2 : com Ex) (pf : compatible e1 e2)
+  | CAtom (c : CAtomic Ex).
+
+Program Fixpoint ceval (Ex : exec_model_consts) (Ext : exec_model_theory Ex) 
+  (c : com Ex) (st : state) : (M Ex state) :=
+  match c with
+  | CDiv _ => id Ex state
+  | CSkip _ => unit Ex st
+  | CSeq _ c1 c2 => 
+      bind Ex (ceval Ex Ext c1 st) (fun st' => ceval Ex Ext c2 st')
+  | CAtom _ ca => ceval_atomic Ex st ca
+  | CPlus_total _ c1 c2 pf => 
+      ap (bop Ex state) (ceval Ex Ext c1 st) (ceval Ex Ext c2 st) _ 
+  | CPlus _ e1 e2 c1 c2 pf => 
+    match veval st e1 with
+    (* | Bval false => (ceval Ex Ext c2 st)  *)
+    | Bval false => match veval st e2 with
+                    | Bval false => id Ex state
+                    | _ => ceval Ex Ext c2 st
+                    end
+    | _ => (ceval Ex Ext c1 st)
+    end
   end.
 
+(* Notations for arithmetic and boolean expressions
+   (These are adapted from the Imp chapter of PLF) *)
+   Coercion avar : string >-> aexp.
+   Coercion Var : string >-> vexp.
+   Coercion num : nat >-> aexp.
+   
+   Declare Custom Entry com.
+   Declare Scope com_scope.
+   
+   Notation "<{ e }>" := e (at level 0, e custom com at level 99) : com_scope.
+   Notation "( x )" := x (in custom com, x at level 99) : com_scope.
+   Notation "x" := x (in custom com at level 0, x constr at level 0) : com_scope.
+   Notation "f x .. y" := (.. (f x) .. y)
+                     (in custom com at level 0, only parsing,
+                     f constr at level 0, x constr at level 9,
+                     y constr at level 9) : com_scope.
+   Notation "x + y"   := (plus x y) (in custom com at level 50, left associativity).
+   Notation "x - y"   := (minus x y) (in custom com at level 50, left associativity).
+   Notation "x * y"   := (mult x y) (in custom com at level 40, left associativity).
+   Notation "'true'"  := true (at level 1).
+   Notation "'true'"  := BTrue (in custom com at level 0).
+   Notation "'false'" := false (at level 1).
+   Notation "'false'" := BFalse (in custom com at level 0).
+   Notation "x <= y"  := (BLe x y) (in custom com at level 70, no associativity).
+   Notation "x > y"   := (BGt x y) (in custom com at level 70, no associativity).
+   Notation "x = y"   := (BEq x y) (in custom com at level 70, no associativity).
+   Notation "x <> y"  := (BNeq x y) (in custom com at level 70, no associativity).
+   Notation "x && y"  := (BAnd x y) (in custom com at level 80, left associativity).
+   Notation "'~' b"   := (BNeg b) (in custom com at level 75, right associativity).
+   
+   (* Now, we define some notations for commands *)
+   Coercion CAtom : CAtomic >-> com.
+   
+   Notation " [ 'div' e ]"  :=
+            (CDiv e) (in custom com at level 0) : com_scope.
+   Notation "[ 'skip' e ]"  :=
+            (CSkip e) (in custom com at level 0) : com_scope.
+   Notation "[ 'assume' Ex ] e "  :=
+             (CAssume Ex e) (in custom com at level 0) : com_scope.
+   Notation "x [:= e ] y "  :=
+            (CAsgn e x y)
+               (in custom com at level 0, x constr at level 0,
+                y at level 85, no associativity) : com_scope.
+   Notation "x [; e ] y " :=
+            (CSeq e x y)
+              (in custom com at level 90, right associativity) : com_scope.
+   Notation "pf -> x [+ e ] y " := 
+            (CPlus_total e x y pf) 
+              (in custom com at level 50, left associativity).
+   Notation "[ e1 c1 ] [+ e ] [ e2 c2 ]" := 
+            (CPlus e e1 e2 c1 c2) 
+              (in custom com at level 50, left associativity).
 
-(*IN PROGRESS*)
-(* Theorem compatible_ceval_plus : forall (Ex : exec_model_consts) 
-  (Ext : exec_model_theory Ex) (st : state) (e1 e2 : vexp) (c1 c2 : com) 
-  (compat_pf : compatible' e1 e2)  (wf1 : wf_com Ex c1) 
-  (wf2 : wf_com Ex c2) (wfc : wf_com Ex 
-  (CPlus (CSeq (CAtom (CAssume e1)) c1) (CSeq (CAtom (CAssume e2)) c2))), 
-  exists wf1' wf2' Hceval,
-  (ceval Ex Ext 
-  (CPlus (CSeq (CAtom (CAssume e1)) c1) (CSeq (CAtom (CAssume e2)) c2)) st wfc)
-  = ap (bop Ex state) (ceval Ex Ext (CSeq (CAtom (CAssume e1)) c1) st wf1')
-    (ceval Ex Ext (CSeq (CAtom (CAssume e2)) c2) st wf2') Hceval.
+Open Scope com_scope.
+
+(* We can then prove that the definition of ceval above is equivalent to the
+   definition using the execution models binary operation *)
+
+Lemma guard_false_implies_id : forall (Ex : exec_model_consts) 
+  (Ext : exec_model_theory Ex) (st : state) (e : vexp) (c : com Ex),
+  veval st e = Bval false ->
+  ceval Ex Ext (CSeq Ex (CAtom Ex (CAssume Ex e)) c) st = id Ex state.
 Proof.
-  intros.
-  remember (wf_atom Ex (CAssume e1)) as wf_assume1.
-  remember (wf_seq Ex (CAtom (CAssume e1)) c1 wf_assume1 wf1) as wf_seq1.
+  intros. simpl. rewrite H. apply (preserve_bind2 Ex Ext).
+Qed.
 
-  remember (wf_atom Ex (CAssume e2)) as wf_assume2.
-  remember (wf_seq Ex (CAtom (CAssume e2)) c2 wf_assume2 wf2) as wf_seq2.
+Theorem compatible_ceval_plus : forall (Ex : exec_model_consts)
+  (Ext : exec_model_theory Ex) (st : state) (e1 e2 : vexp) (c1 c2 : com Ex)
+  (compat : compatible e1 e2),
+  exists H,
+  ceval Ex Ext (CPlus Ex e1 e2 c1 c2 compat) st = 
+  ap (bop Ex state) (ceval Ex Ext (CSeq Ex (CAtom Ex (CAssume Ex e1)) c1) st)
+  (ceval Ex Ext (CSeq Ex (CAtom Ex (CAssume Ex e2)) c2) st) H.
+Proof.
+  intros. unfold compatible in compat.
+  assert (veval st e1 = Bval false \/ veval st e2 = Bval false).
+    { apply compat. }
+  destruct H.
+  - assert (ceval Ex Ext (CSeq Ex (CAtom Ex (CAssume Ex e1)) c1) st = id Ex state).
+      { apply guard_false_implies_id. apply H. }
+    rewrite H0. 
+    assert (exists (Hid : exec_partial Ex state (id Ex state)
+      (ceval Ex Ext (CSeq Ex (CAtom Ex (CAssume Ex e2)) c2) st)),
+      ap (bop Ex state) (id Ex state) 
+      (ceval Ex Ext (CSeq Ex (CAtom Ex (CAssume Ex e2)) c2) st) Hid = 
+      (ceval Ex Ext (CSeq Ex (CAtom Ex (CAssume Ex e2)) c2) st)).
+      { apply (pcm_id_comm Ex Ext). }
+    inversion H1. exists x. rewrite H2. simpl. rewrite H. destruct (veval st e2).
+    + rewrite (bind_of_unit Ex Ext). reflexivity.
+    + destruct b.
+      * rewrite (bind_of_unit Ex Ext). reflexivity.
+      * rewrite (preserve_bind2 Ex Ext). reflexivity.
+  - assert (ceval Ex Ext (CSeq Ex (CAtom Ex (CAssume Ex e2)) c2) st = id Ex state).
+      { simpl. rewrite H. apply (preserve_bind2 Ex Ext). }
+    rewrite H0. 
+    assert (exists (Hid : exec_partial Ex state 
+      (ceval Ex Ext (CSeq Ex (CAtom Ex (CAssume Ex e1)) c1) st) (id Ex state)),
+      ap (bop Ex state) 
+      (ceval Ex Ext (CSeq Ex (CAtom Ex (CAssume Ex e1)) c1) st) (id Ex state) Hid = 
+      (ceval Ex Ext (CSeq Ex (CAtom Ex (CAssume Ex e1)) c1) st)).
+      { apply (pcm_id Ex Ext). }
+    inversion H1. exists x. rewrite H2. simpl. rewrite H. destruct (veval st e1).
+    + rewrite (bind_of_unit Ex Ext). reflexivity.
+    + destruct b.
+      * rewrite (bind_of_unit Ex Ext). reflexivity.
+      * rewrite (preserve_bind2 Ex Ext). reflexivity.
+Qed.
 
-  exists wf_seq1. exists wf_seq2.
 
-  assert (exec_partial Ex state (ceval Ex Ext (CSeq (CAtom (CAssume e1)) c1) st wf_seq1)
-  (ceval Ex Ext (CSeq (CAtom (CAssume e2)) c2) st wf_seq2)).
-  { 
-    apply bop_id_defined. easy. unfold compatible' in compat_pf. 
-    assert (veval st e1 = Bval false \/ veval st e2 = Bval false).
-   { apply compat_pf. } destruct H.
-    - left. rewrite Heqwf_seq1. rewrite Heqwf_assume1. 
-      simpl. rewrite H. apply (preserve_bind2 Ex Ext). 
-      remember (ceval Ex Ext (CSeq (CAtom (CAssume e1)) c1) st wf_seq1) as res.
-      apply res.
-    - right. rewrite Heqwf_seq2. rewrite Heqwf_assume2. 
-    simpl. rewrite H. apply (preserve_bind2 Ex Ext). 
-    remember (ceval Ex Ext (CSeq (CAtom (CAssume e2)) c2) st wf_seq2) as res.
-    apply res.
-  }
-  exists H.
+Theorem partial_proof_irrelevance : forall (Ex : exec_model_consts) (A : Type)
+  (x y : M Ex A) (pf1 pf2 : exec_partial Ex A x y),
+  ap (bop Ex A) x y pf1 = ap (bop Ex A) x y pf2.
+Proof.
+  intros. assert (pf1 = pf2).
+    { apply proof_irrelevance. }
+  rewrite H. reflexivity. 
+Qed.
 
-  unfold compatible' in compat_pf. assert (veval st e1 = Bval false \/ veval st e2 = Bval false).
-   { apply compat_pf. }
-  destruct H0.
-  - assert (ceval Ex Ext (CSeq (CAtom (CAssume e1)) c1) st wf_seq1 = id Ex state).
-    { rewrite Heqwf_seq1. rewrite Heqwf_assume1. simpl. rewrite H0. 
-      apply (preserve_bind2 Ex Ext).  
-      remember (ceval Ex Ext (CSeq (CAtom (CAssume e1)) c1) st wf_seq1) as res.
-      apply res. } destruct wfc.
-      + simpl.
-    replace (ceval Ex Ext (CSeq (CAtom (CAssume e1)) c1) st wf_seq1) with 
-    (id Ex state). *)
-    
+
+Theorem compatible_ceval_plus_rev : forall (Ex : exec_model_consts)
+  (Ext : exec_model_theory Ex) (st : state) (e1 e2 : vexp) (c1 c2 : com Ex)
+  (compat : compatible e1 e2) {H},
+  ap (bop Ex state) (ceval Ex Ext (CSeq Ex (CAtom Ex (CAssume Ex e1)) c1) st)
+  (ceval Ex Ext (CSeq Ex (CAtom Ex (CAssume Ex e2)) c2) st) H =
+  ceval Ex Ext (CPlus Ex e1 e2 c1 c2 compat) st.
+Proof.
+  intros. generalize dependent H. 
+  assert (exists H,
+    ceval Ex Ext (CPlus Ex e1 e2 c1 c2 compat) st = 
+    ap (bop Ex state) (ceval Ex Ext (CSeq Ex (CAtom Ex (CAssume Ex e1)) c1) st)
+    (ceval Ex Ext (CSeq Ex (CAtom Ex (CAssume Ex e2)) c2) st) H).
+    { apply compatible_ceval_plus. }
+  inversion H.
+  rewrite H0. intros. apply partial_proof_irrelevance.
+Qed.
