theories/assertions.v
@@ -1,0 +1,154 @@
+Require Import commands.
+Require Import partial.
+
+Definition assertion (Ex : exec_model_consts) := M Ex state -> Prop.
+
+(* Reorder the arguments of ceval to use in bind *)
+Definition ceval' (Ex : exec_model_consts) (Ext : exec_model_theory Ex) 
+  (c : com) (wfc : wf_com Ex c) (st : state) :=
+  ceval Ex Ext c st wfc. 
+
+(* Define the monadic lifting of denotational semantics (ceval) *)
+Definition ceval_lifted (Ex : exec_model_consts) (Ext : exec_model_theory Ex)
+  (c : com) (st : M Ex state) (wfc : wf_com Ex c) :=
+  bind Ex st (ceval' Ex Ext c wfc).
+
+Definition outcome_triple (Ex : exec_model_consts) (Ext : exec_model_theory Ex)
+  (phi : assertion Ex) (c : com) (wfc : wf_com Ex c) (psi : assertion Ex) := 
+  forall (m : M Ex state),
+  phi m -> psi (ceval_lifted Ex Ext c m wfc).
+
+(* Notations *)
+Declare Scope OL_scope.
+Open Scope OL_scope.
+
+Notation "< phi > c wfc Ex Ext < psi >" :=
+  (outcome_triple Ex Ext phi c wfc psi) (at level 90, psi at next level)
+  : OL_scope.
+
+(* Next, we define the different BI assertions that an outcome assertion can be *)
+Definition Top (Ex : exec_model_consts) : assertion Ex := 
+  fun (m : M Ex state) => True.
+
+Definition Bot (Ex : exec_model_consts) : assertion Ex := 
+  fun (m : M Ex state) => False.
+
+Definition T_plus (Ex : exec_model_consts) : assertion Ex :=
+  fun (m : M Ex state) => m = id Ex state.
+
+Definition AndOC (Ex : exec_model_consts)  (P Q : assertion Ex) : assertion Ex :=
+  fun (m : M Ex state) => P m /\ Q m.
+
+Definition OPlus (Ex : exec_model_consts) (P Q : assertion Ex) : assertion Ex := 
+  fun (m : M Ex state) => exists (m1 m2 : M Ex state) H, 
+  ap (bop Ex state) m1 m2 H = m /\ P m1 /\ P m2.
+
+Definition ImpliesOC (Ex : exec_model_consts) (P Q : assertion Ex) : assertion Ex :=
+  fun (m : M Ex state) => forall (m': M Ex state), m = m' -> P m' -> Q m'.
+
+Definition AtomicAssn (Ex : exec_model_consts) (P : M Ex state -> Prop) : assertion Ex :=
+  fun (m : M Ex state) => P m.
+
+(* Defining inference rules *)
+Inductive rule (Ex : exec_model_consts) (Ext : exec_model_theory Ex) :
+  (assertion Ex) -> com -> (assertion Ex) -> Prop :=
+  (* | zero_rule : forall (P : assertion Ex), rule Ex Ext P CDiv (T_plus Ex) *)
+  | one_rule : forall (P : assertion Ex), rule Ex Ext P CSkip P
+  | seq_rule : forall (P Q R : assertion Ex) (c1 c2 : com),
+                rule Ex Ext P c1 Q -> rule Ex Ext Q c2 R ->
+                rule Ex Ext P (CSeq c1 c2) R
+  | split_rule : forall (P1 Q1 P2 Q2 : assertion Ex) (c : com),
+                  rule Ex Ext P1 c Q1 -> rule Ex Ext P2 c Q2 ->
+                  rule Ex Ext (OPlus Ex P1 P2) c (OPlus Ex Q1 Q2)
+  | empty_rule : forall (c : com), rule Ex Ext (T_plus Ex) c (T_plus Ex)
+  | true_rule : forall (P : assertion Ex) (c : com), 
+                  rule Ex Ext P c (Top Ex)
+  | false_rule : forall (P : assertion Ex) (c : com),
+                  rule Ex Ext (Bot Ex) c P
+  | consequence_rule : forall (P' P Q Q' : assertion Ex) (c : com),
+                    forall (m : M Ex state), ImpliesOC Ex P' P m ->
+                    rule Ex Ext P c Q ->
+                    forall (m : M Ex state), ImpliesOC Ex Q Q' m ->
+                    rule Ex Ext P' c Q'
+  | plus_rule : forall (P Q1 Q2 : assertion Ex) (c1 c2 : com),
+                  rule Ex Ext P c1 Q1 -> rule Ex Ext P c2 Q2 ->
+                  rule Ex Ext P (CPlus c1 c2) (OPlus Ex Q1 Q2).
+
+
+(*---------------- Soundness of Inference Rules ----------------*)
+(* We now begin proving the soundness of Outcome Logic. To begin,
+   we show that the conclusion of every inference rule is a valid
+   outcome triple given the premises and vice versa. *)
+
+   (*
+   <P>*)
+
+Lemma wf_seq_eq : forall (Ex : exec_model_consts)  (c1 c2 : com)
+  (wfc : wf_com Ex (CSeq c1 c2)), 
+  exists (wfc1 : wf_com Ex c1) (wfc2 : wf_com Ex c2),
+    wfc = wf_seq Ex c1 c2 wfc1 wfc2.
+Proof.
+  intros. eexists. eexists.
+  Admitted.
+
+
+Theorem OL_sound : forall (Ex : exec_model_consts) (Ext : exec_model_theory Ex)
+  (P Q : assertion Ex) (c : com) (wfc : wf_com Ex c),
+  rule Ex Ext P c Q -> outcome_triple Ex Ext P c wfc Q.
+Proof.
+  (* intros. induction H.
+  - admit.
+  - unfold outcome_triple ; intros. unfold ceval_lifted ; unfold ceval'.
+    destruct wfc ; simpl. 
+    + simpl. 
+    unfold outcome_triple.
+  - intros. unfold ceval_lifted ; unfold ceval'. destruct wfc.
+   intros. unfold ceval.
+   + unfold T_plus.
+
+   intros ; unfold ceval_lifted ; 
+  unfold ceval' ; simpl ; try contradiction.
+  - destruct wfc ; unfold T_plus ; simpl ; try contradiction.
+    +     *)
+  Admitted.
+
+
+
+(*------------------------ Generic Rules ------------------------*)
+
+(* ONE Rule:
+
+    -----------------
+      <phi> 1 <phi>
+
+*)
+
+Theorem OL_One : forall (Ex : exec_model_consts) (Ext : exec_model_theory Ex) 
+  (phi : assertion Ex),
+    (* <phi> skip Ex Ext <phi>. *)
+    outcome_triple Ex Ext phi CSkip (wf_skip Ex) phi.
+Proof.
+  intros. unfold outcome_triple. intros. unfold ceval_lifted ; unfold ceval'. 
+  simpl. rewrite (bind_with_unit Ex Ext). apply H.
+Qed. 
+
+Theorem OL_Seq : forall (Ex : exec_model_consts) (Ext : exec_model_theory Ex) 
+  (P Q R : assertion Ex) (c1 c2 : com) (wfc1 : wf_com Ex c1) (wfc2 : wf_com Ex c2),
+    (* <phi> skip Ex Ext <phi>. *)
+    outcome_triple Ex Ext P c1 wfc1 Q ->
+    outcome_triple Ex Ext Q c2 wfc2 R ->
+    outcome_triple Ex Ext P (CSeq c1 c2) (wf_seq Ex c1 c2 wfc1 wfc2) R.
+Proof.
+  intros. unfold outcome_triple in *. intros. unfold ceval_lifted in * ; unfold ceval' in *.
+  simpl. rewrite <- (bind_composition Ex Ext). apply H in H1. 
+  apply H0 in H1. apply H1.
+Qed.
+
+Theorem OL_Div : forall (Ex : exec_model_consts) (Ext : exec_model_theory Ex) 
+  (phi : assertion Ex),
+    (* <phi> skip Ex Ext <phi>. *)
+    outcome_triple Ex Ext phi CDiv (wf_div Ex) (T_plus Ex).
+Proof.
+  intros. unfold outcome_triple. intros. unfold ceval_lifted ; unfold ceval'. 
+  simpl. unfold T_plus. 
+Qed. 
