theories/assertions_v2.v
@@ -1,0 +1,488 @@
+Require Import examples.
+Require Import partial.
+Require Import commands.
+From Coq Require Import Ensembles.
+From Coq Require Import Logic.FunctionalExtensionality.
+
+
+Definition assertion (Ex : exec_model_consts) := M Ex state -> Prop.
+
+(* Define the monadic lifting of denotational semantics (ceval) *)
+Definition ceval_lifted (Ex : exec_model_consts) (Ext : exec_model_theory Ex)
+  (c : com Ex) (st : M Ex state) :=
+  bind Ex st (ceval Ex Ext c).
+
+Definition outcome_triple (Ex : exec_model_consts) (Ext : exec_model_theory Ex)
+  (phi : assertion Ex) (c : com Ex) (psi : assertion Ex) := 
+  forall (m : M Ex state),
+  phi m -> psi (ceval_lifted Ex Ext c m).
+
+(* Notations *)
+Declare Scope OL_scope.
+Open Scope OL_scope.
+
+Notation "< phi > c Ex Ext < psi >" :=
+  (outcome_triple Ex Ext phi c psi) (at level 90, psi at next level)
+  : OL_scope.
+
+(* Next, we define the different BI assertions that an outcome assertion can be *)
+Definition Top (Ex : exec_model_consts) : assertion Ex := 
+  fun (m : M Ex state) => True.
+
+Definition Bot (Ex : exec_model_consts) : assertion Ex := 
+  fun (m : M Ex state) => False.
+
+Definition T_plus (Ex : exec_model_consts) : assertion Ex :=
+  fun (m : M Ex state) => m = id Ex state.
+
+Definition AndOC (Ex : exec_model_consts)  (P Q : assertion Ex) : assertion Ex :=
+  fun (m : M Ex state) => P m /\ Q m.
+
+Definition OrOC (Ex : exec_model_consts)  (P Q : assertion Ex) : assertion Ex :=
+  fun (m : M Ex state) => P m \/ Q m.
+
+Definition OPlus (Ex : exec_model_consts) (P Q : assertion Ex) : assertion Ex := 
+  fun (m : M Ex state) => exists (m1 m2 : M Ex state) H, 
+  ap (bop Ex state) m1 m2 H = m /\ P m1 /\ Q m2.
+
+Definition ImpliesOC (Ex : exec_model_consts) (P Q : assertion Ex) : assertion Ex :=
+  fun (m : M Ex state) => forall (m': M Ex state), m = m' -> P m' -> Q m'.
+
+Definition AtomicAssn (Ex : exec_model_consts) (P : M Ex state -> Prop) : assertion Ex :=
+  fun (m : M Ex state) => P m.
+
+(* Defining inference rules *)
+Inductive rule (Ex : exec_model_consts) (Ext : exec_model_theory Ex) :
+  (assertion Ex) -> (com Ex) -> (assertion Ex) -> Prop :=
+  (* | zero_rule : forall (P : assertion Ex), rule Ex Ext P (CDiv Ex) (T_plus Ex) *)
+  | one_rule : forall (P : assertion Ex), rule Ex Ext P (CSkip Ex) P
+  | seq_rule : forall (P Q R : assertion Ex) (c1 c2 : com Ex),
+                rule Ex Ext P c1 Q -> rule Ex Ext Q c2 R ->
+                rule Ex Ext P (CSeq Ex c1 c2) R
+  | split_rule : forall (P1 Q1 P2 Q2 : assertion Ex) (c : com Ex),
+                  rule Ex Ext P1 c Q1 -> rule Ex Ext P2 c Q2 ->
+                  rule Ex Ext (OPlus Ex P1 P2) c (OPlus Ex Q1 Q2)
+  | empty_rule : forall (c : com Ex), rule Ex Ext (T_plus Ex) c (T_plus Ex)
+  | true_rule : forall (P : assertion Ex) (c : com Ex), 
+                  rule Ex Ext P c (Top Ex)
+  | false_rule : forall (P : assertion Ex) (c : com Ex),
+                  rule Ex Ext (Bot Ex) c P
+  | consequence_rule : forall (P' P Q Q' : assertion Ex) (c : com Ex),
+                    (forall (m : M Ex state), ImpliesOC Ex P' P m) ->
+                    rule Ex Ext P c Q ->
+                    (forall (m : M Ex state), ImpliesOC Ex Q Q' m) ->
+                    rule Ex Ext P' c Q'
+  | plus_rule_total : forall (P Q1 Q2 : assertion Ex) (c1 c2 : com Ex) (pf : is_total Ex),
+                      rule Ex Ext P c1 Q1 -> rule Ex Ext P c2 Q2 ->
+                      rule Ex Ext P (CPlus_total Ex c1 c2 pf) (OPlus Ex Q1 Q2)
+  | plus_rule : forall (P Q1 Q2 : assertion Ex) (e1 e2 : vexp) (c1 c2 : com Ex)
+                  (pf : compatible e1 e2),
+                  rule Ex Ext P (CSeq Ex (CAssume Ex e1) c1) Q1 -> 
+                  rule Ex Ext P (CSeq Ex (CAssume Ex e2) c2) Q2 ->
+                  rule Ex Ext P (CPlus Ex e1 e2 c1 c2 pf) (OPlus Ex Q1 Q2).
+
+
+(*---------------- Soundness of Inference Rules ----------------*)
+(* We now begin proving the soundness of Outcome Logic. To begin,
+   we show that the conclusion of every inference rule is a valid
+   outcome triple given the premises and vice versa. *)
+
+(* Lemma assume_to_plus : forall (Ex : exec_model_consts) (Ext : exec_model_theory Ex)
+  (e1 e2 : vexp) (c1 c2 : com Ex) (m : M Ex state) (pf : compatible e1 e2) {H},
+  ap (bop Ex state) (bind Ex m (ceval Ex Ext (CSeq Ex (CAtom Ex (CAssume Ex e1)) c1)))
+  (bind Ex m (ceval Ex Ext (CSeq Ex (CAtom Ex (CAssume Ex e1)) c1))) H = 
+  bind Ex m (ceval Ex Ext (CPlus Ex e1 e2 c1 c2 pf)).
+Proof.
+  intros.  *)
+
+Lemma compatible_addition_defined : forall (Ex : exec_model_consts)
+  (Ext : exec_model_theory Ex) (e1 e2 : vexp) (c1 c2 : com Ex)
+  (pf : compatible e1 e2) (st : state) ,
+  exec_partial Ex state
+  (ceval Ex Ext (CSeq Ex (CAtom Ex (CAssume Ex e1)) c1) st)
+  (ceval Ex Ext (CSeq Ex (CAtom Ex (CAssume Ex e2)) c2) st).
+Proof.
+  intros. unfold compatible in pf. specialize (pf st).
+  destruct pf ; apply (bop_id_defined Ex Ext).
+  - left. simpl. rewrite H. apply (preserve_bind2 Ex Ext).
+  - right. simpl. rewrite H. apply (preserve_bind2 Ex Ext).
+Qed.
+
+
+Theorem OL_sound : forall (Ex : exec_model_consts) (Ext : exec_model_theory Ex)
+  (P Q : assertion Ex) (c : com Ex),
+  rule Ex Ext P c Q -> outcome_triple Ex Ext P c Q.
+Proof.
+  intros. induction H ; unfold outcome_triple in * ; intros ; 
+  unfold ceval_lifted in * ; simpl.
+  - rewrite (bind_with_unit Ex Ext). apply H.
+  - rewrite <- (bind_composition Ex Ext). apply IHrule1 in H1. 
+    apply IHrule2 in H1. apply H1.
+  - unfold OPlus in *. inversion H1. inversion H2. inversion H3. clear H1 H2 H3.
+    destruct H4. destruct H2. remember (ceval_lifted Ex Ext c x) as m1. 
+    remember (ceval_lifted Ex Ext c x0) as m2. exists m1. exists m2. 
+    assert (exists (pf : exec_partial Ex state m1 m2), bind Ex (ap (bop Ex state) x x0 x1) (ceval Ex Ext c) 
+              = ap (bop Ex state) m1 m2 pf).
+      { subst. unfold ceval_lifted. apply (preserve_bind1 Ex Ext). }
+    rewrite H1 in H4. inversion H4. exists x2.
+    split ; try split.
+    + symmetry. easy.
+    + subst. apply IHrule1 in H2. apply H2.
+    + subst. apply IHrule2 in H3. apply H3.
+  - unfold T_plus in *. rewrite H. rewrite (preserve_bind2 Ex Ext) ; easy.
+  - unfold Top. easy.
+  - unfold Bot in H. easy.
+  - unfold ImpliesOC in *. apply H with (m := m) in H2. apply IHrule in H2. 
+    apply H1 with (m := bind Ex m (ceval Ex Ext c)) in H2. apply H2. 
+    reflexivity. reflexivity.
+  - unfold OPlus. assert (Q2 (bind Ex m (ceval Ex Ext c2))). 
+      { apply IHrule2. apply H1. } apply IHrule1 in H1. 
+    remember (ceval_lifted Ex Ext c1 m) as m1. 
+    remember (ceval_lifted Ex Ext c2 m) as m2.
+    exists m1. exists m2.
+    assert (exists H, ap (bop Ex state) m1 m2 H = 
+        bind Ex m (fun st => ap (bop Ex state) ((ceval Ex Ext c1) st) 
+        ((ceval Ex Ext c2) st)  (commands.ceval_obligation_1 ceval Ex Ext st c1 c2 pf))).
+        { intros. subst. apply (preserve_bind3 Ex Ext). }
+    inversion H3. exists x. split. apply H4. split.
+      + subst. unfold ceval_lifted. apply H1.
+      + subst. unfold ceval_lifted. apply H2.
+  - unfold OPlus. unfold compatible in pf. eexists. eexists.
+
+    specialize (compatible_addition_defined Ex Ext e1 e2 c1 c2 pf). intros.
+
+    assert (exists H', ap (bop Ex state) 
+      (bind Ex m (ceval Ex Ext (CSeq Ex (CAtom Ex (CAssume Ex e1)) c1)))
+      (bind Ex m (ceval Ex Ext (CSeq Ex (CAtom Ex (CAssume Ex e2)) c2))) H' =
+      bind Ex m (fun st => ap (bop Ex state) 
+      (ceval Ex Ext (CSeq Ex (CAtom Ex (CAssume Ex e1)) c1) st) 
+      (ceval Ex Ext (CSeq Ex (CAtom Ex (CAssume Ex e2)) c2) st) (H2 st))).
+      { apply (preserve_bind3 Ex Ext). }
+  
+  inversion H3.
+
+  exists x.
+  split ; try split.
+  2: apply IHrule1. 2: apply H1.  
+  2: apply IHrule2. 2: apply H1.
+
+  rewrite H4. assert ((fun (st : state) => ap (bop Ex state) 
+    (ceval Ex Ext (CSeq Ex (CAtom Ex (CAssume Ex e1)) c1) st)
+    (ceval Ex Ext (CSeq Ex (CAtom Ex (CAssume Ex e2)) c2) st) (H2 st)) = 
+    (fun (st : state) => ceval Ex Ext (CPlus Ex e1 e2 c1 c2 pf) st)).
+
+    (* Is there a way to do this w/o funcitonal extensionality? *)
+    { apply functional_extensionality. intros. apply compatible_ceval_plus_rev. }
+
+    rewrite H5. simpl. reflexivity.
+Qed.
+
+
+(*--------------------- Subsumption of Hoare Logic ---------------------*)
+
+(* Before proving that OL subsumes Hoare Logic, we first need to define
+   the notions of under-approximation and partial correctness *)
+
+(* Partial correctness *)
+Definition pc (Ex : exec_model_consts) (Ext : exec_model_theory Ex)
+  (P : assertion Ex) (c : com Ex) (Q : assertion Ex) :=
+  outcome_triple Ex Ext P c (OrOC Ex Q (T_plus Ex)).
+
+(* We will now show that OL, when instantiated using the powerset monad,
+   subsumes Hoare Logic *)
+
+Definition PS := powerset_exec_model.
+Definition PSt := powerset_exec_model_theory.
+
+Definition hoare_triple (P : state -> Prop) (c : com PS) (Q : state -> Prop) :=
+  forall (st st': state),
+  P (st) -> In state (ceval PS PSt c st) st' -> Q (st').
+
+Notation "{{ P }} c {{ Q }}" :=
+  (hoare_triple P c Q) (at level 90, P at next level)
+  : OL_scope.
+
+
+(* Defining atomic assertions for the powerset model *)
+Definition atomic_powerset (P : state -> Prop) : assertion PS :=
+  fun (A : Ensemble state) => Inhabited state A  /\
+    forall (x : state), In state A x -> P x.
+
+
+(* Proving subsumption of Hoare Logic *)
+
+Lemma apply_f_to_uninhabited : forall (A B : Type) (U : Ensemble A) (f : A -> Ensemble B),
+  ~ Inhabited A U -> ~ Inhabited B (apply_f U f).
+Proof.
+  intros. unfold apply_f. unfold not in *. intros. apply H. inversion H0.
+  inversion H1. destruct H2. econstructor. apply H2.
+Qed.
+
+Lemma ap_union : forall (U T : Ensemble state) (pf : exec_partial PS state U T),
+  ap (partial_union state) U T pf = Union state U T. 
+Proof.
+  intros. apply Extensionality_Ensembles. unfold Same_set. unfold Included. 
+  split ; intros.
+  - unfold In in *. unfold partial_union in H. unfold make_partial in H.
+    unfold ap in H. easy.
+  - unfold In in *. unfold partial_union. unfold make_partial. unfold ap. easy.
+Qed. 
+
+
+Lemma assume_inhabited_or_not : forall (e : vexp) (U : Ensemble state),
+  Inhabited state U -> 
+  Inhabited state (apply_f U (ceval PS PSt (CAtom PS (CAssume PS e)))) \/
+  not (Inhabited state (apply_f U (ceval PS PSt (CAssume PS e)))).
+Proof.
+  intros. simpl. inversion H. unfold In in H0. destruct (veval x e) eqn:res.
+  - left. unfold apply_f. exists x. exists x. split. apply H0. rewrite res.
+    apply In_singleton.
+  - destruct b.
+    + unfold apply_f. left. eexists. exists x. split. apply H0. unfold In.
+      rewrite res. apply In_singleton.
+    + 
+
+Admitted.
+
+Lemma seq_inhabited_or_not : forall (U : Ensemble state) (c1 c2 : com PS),
+  Inhabited state U -> 
+  (forall U', Inhabited state U' -> 
+    Inhabited state (apply_f U' (ceval PS PSt c1)) \/ 
+    not (Inhabited state (apply_f U' (ceval PS PSt c1)))) ->
+  (forall U', Inhabited state U' -> 
+    Inhabited state (apply_f U' (ceval PS PSt c2)) \/ 
+    not (Inhabited state (apply_f U' (ceval PS PSt c2)))) ->
+  Inhabited state (apply_f U (ceval PS PSt (CSeq PS c1 c2))) \/ 
+    not (Inhabited state (apply_f U (ceval PS PSt (CSeq PS c1 c2)))).
+Proof.
+  intros. apply H0 in H. destruct H.
+  + apply H1 in H. destruct H.
+    * left. simpl. rewrite <- (bind_composition PS PSt). apply H.
+    * right. simpl.  rewrite <- (bind_composition PS PSt). apply H.
+  + right. simpl. rewrite <- (bind_composition PS PSt). apply apply_f_to_uninhabited.
+    apply H.
+Qed.
+  
+
+Lemma apply_f_inhabited: forall (U : Ensemble state) (c : com PS),
+  Inhabited state U -> Inhabited state (apply_f U (ceval PS PSt c)) \/  
+  not (Inhabited state (apply_f U (ceval PS PSt c))).
+Proof.
+  intros. generalize dependent U. induction c ; intros.
+  - simpl. right. unfold not. intros. unfold apply_f in H0. inversion H0. 
+    unfold In in H1. inversion H1. inversion H2. contradiction.
+  - left. inversion H. unfold apply_f. simpl. unfold In. exists x.
+    unfold In in H0. unfold In. exists x. split ; auto. constructor.
+  - apply seq_inhabited_or_not ; easy.
+  - assert (H' := H). apply IHc1 in H. apply IHc2 in H'. destruct H.
+    + left. simpl. unfold apply_f. unfold In. inversion H. unfold apply_f in H0.
+      unfold In in H0. inversion H0. destruct H1. exists x. unfold In. exists x0.
+      split. apply H1. rewrite ap_union. apply Union_introl. apply H2.
+    + destruct H'.
+      * left. simpl. unfold apply_f. unfold In. inversion H0. unfold apply_f in H1.
+        unfold In in H1. inversion H1. destruct H2. exists x. unfold In. exists x0.
+        split. apply H2. rewrite ap_union. apply Union_intror. apply H3.
+      * right. unfold not. unfold not in H. unfold not in H0. intros. inversion H1.
+        unfold In in H2. unfold apply_f in H2. unfold In in H2. inversion H2.
+        destruct H3. simpl in H4. rewrite ap_union in H4. destruct H4. 
+        -- apply H. unfold apply_f. exists x. unfold In. exists x0. split. 
+           apply H3. apply H4.
+        -- apply H0. unfold apply_f. exists x. unfold In. exists x0. split.
+           apply H3. apply H4.
+  - specialize (compatible_addition_defined PS PSt e1 e2 c1 c2 pf). intros.
+    assert (ceval PS PSt (CPlus PS e1 e2 c1 c2 pf) = 
+      fun st => ap (bop PS state) 
+      (ceval PS PSt (CSeq PS (CAtom PS (CAssume PS e1)) c1) st)
+      (ceval PS PSt (CSeq PS (CAtom PS (CAssume PS e2)) c2) st) (H0 st)).
+      { apply functional_extensionality. intros. 
+        rewrite compatible_ceval_plus_rev with (compat := pf). reflexivity. }
+      rewrite H1.
+
+    remember (ceval PS PSt (CSeq PS (CAtom PS (CAssume PS e1)) c1)) as f1.
+    remember (ceval PS PSt (CSeq PS (CAtom PS (CAssume PS e2)) c2)) as f2.
+
+    specialize (preserve_bind3 PS PSt state state f1 f2 U H0). intros.
+    inversion H2. simpl in H3. simpl. rewrite <- H3. rewrite ap_union.
+    clear H3 x H2 H1 H0.
+    
+    specialize (assume_inhabited_or_not e1) as He1. 
+    specialize (assume_inhabited_or_not e2) as He2.
+    specialize (seq_inhabited_or_not U (CAtom PS (CAssume PS e1)) 
+      c1 H He1 IHc1) as Hguard1. 
+    specialize (seq_inhabited_or_not U (CAtom PS (CAssume PS e2)) 
+      c2 H He2 IHc2) as Hguard2.
+    
+    destruct Hguard1.
+    + left. inversion H0. exists x. subst f1. apply Union_introl. apply H1.
+    + destruct Hguard2 ; subst f2.
+      * left. inversion H1. exists x. apply Union_intror. apply H2.
+      * right. unfold not. intros. inversion H2. inversion H3.
+        subst f1. unfold not in H0. apply Inhabited_intro in H4. apply H0 in H4.
+        apply H4.
+        unfold not in H1. apply Inhabited_intro in H4. apply H1 in H4. apply H4.
+    
+  - destruct c.
+    + apply assume_inhabited_or_not. apply H.
+    + unfold apply_f. inversion H. unfold In in *. left. eexists. exists x0.
+      split. apply H0. simpl. apply In_singleton.
+Qed.  
+
+
+Lemma not_inhabited_empty : forall (A : Type) (U : Ensemble A),
+  not (Inhabited A U) -> U = Empty_set A.
+Proof.
+  intros. apply Extensionality_Ensembles. unfold Same_set. split.
+  - unfold Included. intros. unfold not in H. exfalso. apply H. econstructor.
+    apply H0.
+  - unfold Included. intros. unfold not in H. unfold In in H0. contradiction.
+Qed. 
+
+Lemma inhabited_not_empty : forall (A : Type) (U : Ensemble A),
+  Inhabited A U -> U <> Empty_set A.
+Proof.
+  intros. unfold not. intros. subst. inversion H. inversion H0.
+Qed.
+
+(* Now proving the theorem itself *)
+Theorem OL_subsumes_HL : forall (P Q : state -> Prop) (c : com PS),
+  hoare_triple P c Q <-> pc PS PSt (atomic_powerset P) c (atomic_powerset Q).
+Proof.
+  intros. unfold pc. unfold outcome_triple. unfold hoare_triple. unfold atomic_powerset. split.
+  - intros. unfold OrOC. unfold ceval_lifted. simpl. inversion H0.  
+    apply apply_f_inhabited with (c := c) in H1.
+    destruct H1.
+    + left. split. apply H1. intros. unfold apply_f in H3. inversion H3. 
+      apply H with (st := x0) (st' := x). apply H2. apply H4. apply H4.
+    + right. unfold T_plus.  apply not_inhabited_empty in H1. rewrite H1.
+      reflexivity.
+  - intros. assert (atomic_powerset P (Singleton state st)).
+      { unfold atomic_powerset. split. assert (In state (Singleton state st) st).
+        {  apply In_singleton. } apply Inhabited_intro in H2. apply H2. intros.
+        inversion H2. rewrite <- H3. easy. }
+    apply H in H2. unfold OrOC in H2. destruct H2. 
+
+    (* Case where C[{st}] |= Q *)
+    + destruct H2. apply H3. simpl. unfold In. unfold apply_f. exists st. split.
+      apply In_singleton. apply H1.
+
+    (* Case where C[{st}] |= T^+ *)
+    + unfold T_plus in H2. simpl in H2. unfold apply_f in H2. 
+      assert ((ceval PS PSt c st) = Empty_set state). 
+      { rewrite <- H2. apply Extensionality_Ensembles. unfold Same_set. split.
+        - unfold Included. intros. unfold In. exists st. split. apply In_singleton.
+          unfold In in H3. apply H3.
+        - unfold Included. intros. unfold In. destruct H3. destruct H3.
+          inversion H3. subst. unfold In in H4. apply H4. }
+      apply Inhabited_intro in H1. apply inhabited_not_empty in H1. contradiction.
+Qed.
+
+
+(* -------------------- Subsumption of Lisbon Logic -------------------- *)
+(* We will now show that OL subsumes Lisbon Logic. For this, we will re-use
+   some of the definitions from the above section along with some new ones.
+   most notably, we describe the semantics of a triple in Lisbon Logic: *)
+      
+(* Under-approximation *)
+Definition under (Ex : exec_model_consts) (Ext : exec_model_theory Ex)
+  (P : assertion Ex) (c : com Ex) (Q : assertion Ex) :=
+  outcome_triple Ex Ext P c (OPlus Ex Q (Top Ex)).
+
+Definition lisbon_triple (P : state -> Prop) (c : com PS) (Q : state -> Prop) :=
+  forall st,
+  P (st) -> exists st', In state (ceval PS PSt c st) st' /\ Q (st').
+
+
+Lemma ceval_linear : forall (X Y Z : M PS state) (c : com PS) {H},
+  Union state X Y = Z -> 
+  ap (bop PS state) (ceval_lifted PS PSt c X) (ceval_lifted PS PSt c Y) H =
+  ceval_lifted PS PSt c Z.
+Proof.
+  intros. unfold ceval_lifted. rewrite <- H0.
+  assert (exists H, ap (bop PS state) X Y H = Union state X Y).
+    { eexists. reflexivity. }
+  inversion H1. rewrite <- H2. 
+  assert (exists H, bind PS (ap (bop PS state) X Y x) (ceval PS PSt c) = 
+                    ap (bop PS state) (bind PS X (ceval PS PSt c)) 
+                    (bind PS Y (ceval PS PSt c)) H).
+    { apply (preserve_bind1 PS PSt). }
+  inversion H3. rewrite H4. reflexivity. 
+  Unshelve. simpl. unfold powerset_partial. tauto.
+Qed.
+
+
+Lemma exists_satisfies_under : forall (X : Ensemble state) (P : state -> Prop),
+  OPlus PS (atomic_powerset P) (Top PS) X <-> exists x, In state X x /\ P x.
+Proof.
+  intros. split.
+  - intros. unfold OPlus in H. inversion H. inversion H0. inversion H1. 
+    destruct H2. destruct H3. unfold atomic_powerset in H3. destruct H3.
+    inversion H3. exists x2. 
+    assert (X = Union state x x0).
+      { rewrite <- H2. reflexivity. } 
+    split. rewrite H7. apply Union_introl. apply H6. apply H5. apply H6.
+  - intros. inversion H. destruct H0. unfold OPlus. 
+    remember (Singleton state x) as s. exists s. exists X. exists I. split.
+    + assert (ap (bop PS state) s X I = Union state s X).
+        { simpl. reflexivity. }
+      rewrite H2. apply Extensionality_Ensembles. unfold Same_set. unfold Included.
+      split.
+      * intros. destruct H3. subst. inversion H3. rewrite <- H4. apply H0. apply H3.
+      * intros. apply Union_intror. apply H3.
+    + split. unfold atomic_powerset.
+      * split. assert (In state s x). { subst. apply In_singleton. } 
+        apply Inhabited_intro in H2. apply H2. intros. subst. inversion H2.
+        rewrite <- H3. apply H1.
+      * unfold Top. tauto.
+Qed.
+
+
+Lemma PS_bop_union : forall (X Y : Ensemble state) {H},
+  ap (bop PS state) X Y H = Union state X Y.
+Proof. 
+  intros. simpl. reflexivity.
+Qed.
+
+
+Lemma apply_f_singleton : forall (st : state) (f : state -> Ensemble state),
+  apply_f (Singleton state st) f = f st.
+Proof.
+  intros. apply Extensionality_Ensembles. unfold Same_set. unfold Included.
+  unfold apply_f.
+  split ; intros.
+  - inversion H. destruct H0. inversion H0. apply H1.
+  - exists st. split. apply In_singleton. apply H.
+Qed.
+
+
+Theorem OL_subsumes_LL : forall (P Q : state -> Prop) (c : com PS),
+  lisbon_triple P c Q <-> under PS PSt (atomic_powerset P) c (atomic_powerset Q).
+Proof.
+  intros. unfold under. unfold outcome_triple. unfold lisbon_triple. split.
+  (* Forwards Direction *)
+  - intros. destruct H0. inversion H0. specialize (H1 x H2). 
+    specialize (H x H1). inversion H. destruct H3. remember (Singleton state x) as s.
+    apply exists_satisfies_under. exists x0. split.
+    + assert (Union state s m = m).
+        { subst. apply Extensionality_Ensembles. unfold Same_set. unfold Included.
+          split ; intros. destruct H5. subst. inversion H5. rewrite <- H6. 
+          apply H2. apply H5. apply Union_intror. apply H5. }
+      assert (ap (bop PS state) (ceval_lifted PS PSt c s) (ceval_lifted PS PSt c m) I =
+              (ceval_lifted PS PSt c m)).
+        { apply ceval_linear. apply H5. }
+      rewrite <- H6.
+      assert (ceval PS PSt c x = ceval_lifted PS PSt c s ).
+            { rewrite <- apply_f_singleton. simpl. subst. reflexivity. }
+      rewrite <- H7.  rewrite PS_bop_union. apply Union_introl. easy.
+    + apply H4.
+  (* Backwards Direction *)
+  - intros. remember (Singleton state st) as s.
+    specialize (H s). assert (atomic_powerset P s).
+      { unfold atomic_powerset. split. assert (In state s st). subst. 
+        apply In_singleton. apply Inhabited_intro in H1. apply H1.
+        intros. subst. inversion H1. rewrite <- H2. apply H0. }
+    apply H in H1. apply exists_satisfies_under in H1. inversion H1. destruct H2.
+    exists x. split.
+    + rewrite <- apply_f_singleton. unfold ceval_lifted in H2. simpl in H2.
+      subst. apply H2.
+    + apply H3. 
+Qed.
